Proved NFA -> epsNFA construction, finished regex -> DFA (now the hard part)

src/automata/epsnfa.lean
@@ -77,6 +77,8 @@ begin
     }
 end
 
+section epsnfa_to_nfa
+
 def epsnfa_to_nfa (enfa : epsNFA S Q) : nfa.NFA S Q := {
     start := enfa.start,
     term := {x | eps_reach enfa x enfa.term},
@@ -135,5 +137,96 @@ begin
 end
 
 theorem epsnfa_to_dfa_eq {L : set (list S)} : epsnfa_lang L → dfa.dfa_lang L := nfa.nfa_to_dfa_eq ∘ epsnfa_to_nfa_eq
+
+end epsnfa_to_nfa
+
+section nfa_to_epsnfa
+
+inductive U (Q : Type) : Type
+| inside : Q → U
+| finish : U
+
+def nfa_to_epsnfa (nfa : nfa.NFA S Q) : epsNFA S (U Q) := {
+    start := U.inside nfa.start,
+    term := U.finish,
+    next := λ q c, begin
+        cases q,
+        exact U.inside '' nfa.next q c,
+        exact ∅,
+    end,
+    eps := λ q, begin
+        cases q,
+        by_cases q ∈ nfa.term,
+        exact {U.finish},
+        exact ∅,
+        exact ∅,
+    end,
+}
+
+lemma nfa_to_epsnfa_accepts_iff_accepts
+    (n : nfa.NFA S Q) {en : epsNFA S (U Q)} (w : list S) (st : Q)
+    : en = nfa_to_epsnfa n → (go en (U.inside st) w U.finish  ↔ ∃ t : Q, nfa.go n st w t ∧ t ∈ n.term) :=
+begin
+    rintro rfl,
+    split, {
+        intro go_enfa,
+        generalize hst : U.inside st = ust,
+        generalize hfi : (U.finish : U Q) = ufi,
+        rw [hst, hfi] at go_enfa,
+        induction go_enfa generalizing st, {
+            subst hfi,
+            injection hst,
+        }, {
+            substs hst hfi,
+            cases go_enfa_n, {
+                specialize go_enfa_ih rfl go_enfa_n rfl,
+                rcases go_enfa_ih with ⟨t, t_go, t_term⟩,
+                simp [nfa_to_epsnfa] at go_enfa_h,
+                use [t, nfa.go.step go_enfa_h t_go, t_term],
+            }, {
+                simpa [nfa_to_epsnfa] using go_enfa_h,
+            }
+        }, {
+            substs hst hfi,
+            cases go_enfa_n, {
+                by_cases st ∈ n.term;
+                simpa [nfa_to_epsnfa, h] using go_enfa_h,
+            }, {
+                by_cases st ∈ n.term, {
+                    suffices tail_nil : go_enfa_tail = [],
+                    subst tail_nil, 
+                    use [st, nfa.go.finish, h],
+                    cases go_enfa_a, 
+                    { refl, },
+                    { simpa [nfa_to_epsnfa] using go_enfa_a_h, },
+                    { simpa [nfa_to_epsnfa] using go_enfa_a_h, },
+                }, {
+                    simpa [nfa_to_epsnfa, h] using go_enfa_h,
+                }
+            }
+        }
+    }, {
+        rintro ⟨t, t_go, t_term⟩,
+        induction t_go, {
+            refine go.eps _ go.finish,
+            simp [nfa_to_epsnfa, t_term], 
+        }, {
+            refine go.step _ (t_go_ih t_term),
+            simpa [nfa_to_epsnfa],
+        },
+    }
+end
+
+theorem nfa_to_epsnfa_eq {L : set (list S)} : nfa.nfa_lang L → epsnfa_lang L :=
+begin
+    rintro ⟨Q, nfa, rfl⟩,
+    use [U Q, nfa_to_epsnfa nfa],
+    ext x,
+    exact nfa_to_epsnfa_accepts_iff_accepts nfa x nfa.start rfl,
+end
+
+theorem dfa_to_epsnfa_eq {L : set (list S)} : dfa.dfa_lang L → epsnfa_lang L := nfa_to_epsnfa_eq ∘ nfa.dfa_to_nfa_eq
+
+end nfa_to_epsnfa
 
 end epsnfa
